Add subsumption rule.

WebAssembly/Wasm.thy
@@ -86,8 +86,10 @@ inductive b_e_typing :: "[t_context, b_e list, tf] \<Rightarrow> bool" ("_ \<tur
 | empty:"\<C> \<turnstile> [] : ([] _> [])"
   \<comment> \<open>\<open>composition\<close>\<close>
 | composition:"\<lbrakk>\<C> \<turnstile> es : (t1s _> t2s); \<C> \<turnstile> [e] : (t2s _> t3s)\<rbrakk> \<Longrightarrow> \<C> \<turnstile> es @ [e] : (t1s _> t3s)"
-  \<comment> \<open>\<open>weakening\<close>\<close>
-| weakening:"\<C> \<turnstile> es : (t1s _> t2s) \<Longrightarrow> \<C> \<turnstile> es : (ts @ t1s _> ts @ t2s)"
+(*  \<comment> \<open>\<open>weakening\<close>\<close>
+| weakening:"\<C> \<turnstile> es : (t1s _> t2s) \<Longrightarrow> \<C> \<turnstile> es : (ts @ t1s _> ts @ t2s)"*)
+  \<comment> \<open>\<open>subtyping\<close>\<close>
+| subsumption:"\<lbrakk>\<C> \<turnstile> es : tf; instr_subtyping tf tf'\<rbrakk> \<Longrightarrow> \<C> \<turnstile> es : tf'"
 
 | memory_init: "\<lbrakk>length (memory \<C>) \<ge> 1; i < length (data \<C>)\<rbrakk> \<Longrightarrow> \<C> \<turnstile> [Memory_init i] : ([T_num T_i32, T_num T_i32, T_num T_i32] _> [])"
 | memory_copy: "\<lbrakk>length (memory \<C>) \<ge> 1\<rbrakk> \<Longrightarrow> \<C> \<turnstile> [Memory_copy] : ([T_num T_i32, T_num T_i32, T_num T_i32] _> [])"
@@ -162,8 +164,11 @@ and       l_typing :: "[s, (t list) option, f, e list, t list] \<Rightarrow> boo
   "\<C> \<turnstile> b_es : tf \<Longrightarrow> \<S>\<bullet>\<C> \<turnstile> $*b_es : tf"
   (* composition *)
 | "\<lbrakk>\<S>\<bullet>\<C> \<turnstile> es : (t1s _> t2s); \<S>\<bullet>\<C> \<turnstile> [e] : (t2s _> t3s)\<rbrakk> \<Longrightarrow> \<S>\<bullet>\<C> \<turnstile> es @ [e] : (t1s _> t3s)"
-  (* weakening *)
-| "\<S>\<bullet>\<C> \<turnstile> es : (t1s _> t2s) \<Longrightarrow>\<S>\<bullet>\<C> \<turnstile> es : (ts @ t1s _> ts @ t2s)"
+(*  (* weakening *)
+| "\<S>\<bullet>\<C> \<turnstile> es : (t1s _> t2s) \<Longrightarrow> \<S>\<bullet>\<C> \<turnstile> es : (ts @ t1s _> ts @ t2s)"*)
+  (* subsumption *)
+| "\<lbrakk>\<S>\<bullet>\<C> \<turnstile> es : tf; instr_subtyping tf tf'\<rbrakk> \<Longrightarrow> \<S>\<bullet>\<C> \<turnstile> es : tf'"
+
 | "ref_typing \<S> v_r t \<Longrightarrow> \<S>\<bullet>\<C> \<turnstile> [Ref v_r] :([] _> [T_ref t])"
   (* trap *)
 | "\<S>\<bullet>\<C> \<turnstile> [Trap] : tf"
